new/proof/chan_proof/closeable.v
@@ -1,3 +1,4 @@
+From iris.algebra.lib Require Import dfrac_agree.
 Require Import New.proof.proof_prelude.
 
 (** A pattern for channel usage: a channel that never has anything sent, and is
@@ -5,19 +6,19 @@ Require Import New.proof.proof_prelude.
     readers. *)
 Class closeable_chanG Σ :=
   {
-    ghost_var_inG :: ghost_varG Σ ()
+    close_tok_inG :: inG Σ (dfrac_agreeR boolO)
   }.
 
 Record closeable_chan_names :=
   {
-    tok_gn : gname;
+    closed_gn : gname;
     init_len : nat; (* for gauge invariance *)
   }.
 
 Section proof.
 
 Context `{hG: heapGS Σ, !ffi_semantics _ _}.
-Context `{closeable_chanG Σ}.
+Context `{!closeable_chanG Σ}.
 
 (* Note: could make the namespace be user-chosen *)
 Local Definition is_closeable_chan_internal (ch : chan.t) γch (Pclose : iProp Σ) : iProp Σ :=
@@ -27,12 +28,16 @@ Local Definition is_closeable_chan_internal (ch : chan.t) γch (Pclose : iProp �
         "ch" ∷ own_chan ch st ∗
         "%Hempty" ∷ ⌜ length st.(chanstate.sent) = γch.(init_len) ⌝ ∗
         "%Hle" ∷ ⌜ length st.(chanstate.sent) ≤ st.(chanstate.received) ⌝ ∗
-        "#HPclosed" ∷ (if st.(chanstate.closed) then (□ Pclose) else True) ∗
-        "Hclosed" ∷ (if st.(chanstate.closed) then ghost_var γch.(tok_gn) 1 () else True)
+        "#Hclosed" ∷ (if st.(chanstate.closed) then
+                        (□ Pclose ∗ own γch.(closed_gn) (to_dfrac_agree DfracDiscarded true))
+                     else True) ∗
+        "Hopen" ∷ (if st.(chanstate.closed) then True
+                   else own γch.(closed_gn) (to_dfrac_agree (DfracOwn (1/2)) false))
     ).
 
 Definition own_closeable_chan ch Pclose : iProp Σ :=
-  ∃ γch, is_closeable_chan_internal ch γch Pclose ∗ ghost_var γch.(tok_gn) 1 ().
+  ∃ γch, is_closeable_chan_internal ch γch Pclose ∗
+         own γch.(closed_gn) (to_dfrac_agree (DfracOwn (1/2)) false).
 #[global] Opaque own_closeable_chan.
 #[local] Transparent own_closeable_chan.
 
@@ -44,9 +49,17 @@ Definition is_closeable_chan (ch : chan.t) (Pclose : iProp Σ) : iProp Σ :=
 #[global] Instance is_closeable_chan_pers ch P :
   Persistent (is_closeable_chan ch P) := _.
 
+Definition is_closed_chan (ch : chan.t) (Pclose : iProp Σ) : iProp Σ :=
+  ∃ γch, is_closeable_chan_internal ch γch Pclose ∗
+         own γch.(closed_gn) (to_dfrac_agree DfracDiscarded true).
+#[global] Opaque is_closed_chan.
+#[local] Transparent is_closed_chan.
+#[global] Instance is_closed_chan_pers ch P :
+  Persistent (is_closed_chan ch P) := _.
+
 Lemma closeable_chan_receive ch Pclosed Φ :
   is_closeable_chan ch Pclosed -∗
-  (Pclosed -∗ Φ (#(), #false)%V) -∗ receive_atomic_update unit ch Φ.
+  (Pclosed ∗ is_closed_chan ch Pclosed -∗ Φ (#(), #false)%V) -∗ receive_atomic_update unit ch Φ.
 Proof.
   iNamed 1. iIntros "HΦ". rewrite /receive_atomic_update. iFrame "#".
   iInv "Hinv" as "Hi" "Hclose". iApply fupd_mask_intro; [ solve_ndisj | iIntros "Hmask"].
@@ -54,8 +67,8 @@ Proof.
   destruct decide as [|].
   - iIntros "Hch". iFrame.
     iMod "Hmask" as "_". iMod ("Hclose" with "[-HΦ]").
-    { iFrame "∗#%". } iApply "HΦ". destruct st.(chanstate.closed); try done.
-    naive_solver.
+    { iFrame "∗#%". } iApply "HΦ". destruct st.(chanstate.closed); last naive_solver.
+    iDestruct "Hclosed" as "[#$ $]". iFrame "#". done.
   - (* eventually get a contradiction down this path *)
     iIntros "Hch". iMod "Hmask" as "_".
     iMod ("Hclose" with "[-]"). { iFrame "∗#%". iPureIntro. simpl. lia. }
@@ -65,7 +78,7 @@ Proof.
     exfalso. apply lookup_lt_Some in Hbad. lia.
 Qed.
 
-Lemma closeable_chan_nonblocking_receive ch Pclosed Φ Φnotready :
+Lemma own_closeable_chan_nonblocking_receive ch Pclosed Φ Φnotready :
   own_closeable_chan ch Pclosed -∗
   Φnotready -∗ nonblocking_receive_atomic_update unit ch Φ Φnotready.
 Proof.
@@ -73,13 +86,28 @@ Proof.
   iInv "Hinv" as "Hi" "Hclose". iApply fupd_mask_intro; [ solve_ndisj | iIntros "Hmask"].
   iNext. iNamed "Hi". iFrame.
   destruct decide as [|].
-  - destruct a as [-> ?]. iCombine "Hown Hclosed" gives %[Hbad _]. done.
+  - destruct a as [-> ?]. iRight in "Hclosed". iCombine "Hown Hclosed" gives %Hbad.
+    exfalso. rewrite dfrac_agree_op_valid in Hbad. naive_solver.
   - destruct lookup eqn:Hlookup.
     { simpl. apply lookup_lt_Some in Hlookup. word. }
     iFrame.
     iIntros "Hch". iMod "Hmask" as "_".
     iMod ("Hclose" with "[-]"). { iFrame "∗#%". }
     done.
+Qed.
+
+Lemma is_closed_chan_nonblocking_receive ch Pclosed Φ Φnotready :
+  is_closed_chan ch Pclosed -∗
+  Φ (#(), #false)%V -∗ nonblocking_receive_atomic_update unit ch Φ Φnotready.
+Proof.
+  iIntros "(% & H & #His)". iNamed "H". iIntros "HΦ". rewrite /nonblocking_receive_atomic_update. iFrame "#".
+  iInv "Hinv" as "Hi" "Hclose". iApply fupd_mask_intro; [ solve_ndisj | iIntros "Hmask"].
+  iNext. iNamed "Hi". iFrame.
+  destruct decide as [|].
+  - destruct st. destruct a as [? ?]. subst. simpl in *. iIntros "Hch".
+    iFrame. iMod "Hmask". iMod ("Hclose" with "[-]"); last done. iFrame "∗#%".
+  - destruct st. simpl in *. destruct closed; first lia.
+    iCombine "His Hopen" gives %Hbad%dfrac_agree_op_valid. exfalso. naive_solver.
 Qed.
 
 Lemma wp_closeable_chan_close ch Pclosed Φ :
@@ -91,8 +119,11 @@ Proof.
   unshelve wp_apply (wp_chan_close with "[$]"); try tc_solve.
   iInv "Hinv" as "Hi" "Hclose". iApply fupd_mask_intro; [ solve_ndisj | iIntros "Hmask"].
   iNext. iNamed "Hi". iFrame. destruct (st.(chanstate.closed)).
-  { iCombine "Hown Hclosed" gives %Hbad. exfalso. naive_solver. }
+  { iRight in "Hclosed". iCombine "Hown Hclosed" gives %Hbad%dfrac_agree_op_valid. exfalso. naive_solver. }
   iSplitR; first done. iIntros "Hch". iMod "Hmask" as "_".
+  iCombine "Hown Hopen" as "Hown". rewrite -dfrac_agree_op dfrac_op_own Qp.half_half.
+  iMod (own_update _ _ (to_dfrac_agree DfracDiscarded true) with "Hown") as "#H".
+  { apply cmra_update_exclusive. done. }
   iMod ("Hclose" with "[-]"); last done.
   iFrame "∗#%".
 Qed.
@@ -105,12 +136,16 @@ Lemma alloc_closeable_chan {E} Pclose ch (s : chanstate.t unit) :
   own_closeable_chan ch Pclose.
 Proof.
   intros ? Hnotclosed. iIntros "Hch". iDestruct (own_chan_is_chan with "Hch") as "#His".
-  iMod (ghost_var_alloc ()) as (tok_gn) "Htok".
+  iMod (own_alloc
+          ((to_dfrac_agree (DfracOwn (1/2)) false) ⋅ (to_dfrac_agree (DfracOwn (1/2)) false))
+       ) as (tok_gn) "Htok".
+  { rewrite -dfrac_agree_op //. }
+  iDestruct "Htok" as "[Htok Htok2]".
   iAssert (|={E}=> is_closeable_chan_internal ch ltac:(econstructor) Pclose)%I with "[-Htok]" as ">#H".
   2:{ iFrame "∗#". simpl. iFrame. done. }
   simpl. iFrame.
   iMod (inv_alloc with "[-]") as "$"; last done.
-  iFrame. rewrite Hnotclosed. simpl.
+  iFrame. rewrite Hnotclosed. iFrame. simpl.
   iPureIntro. split; [done|lia].
 Qed.
 
